PolyInt/APolyInt.v
@@ -33,7 +33,7 @@ Section S.
 
     Fixpoint termpoly k (t : bterm k) : poly (S k) :=
       match t with
-        | BVar H => ((1)%Z, mxi (gt_le_S (le_lt_n_Sm H))) :: List.nil
+        | BVar H => ((1)%Z, mxi (NatCompat.gt_le_S (NatCompat.le_lt_n_Sm H))) :: List.nil
         | BFun f v => pcomp (PI f) (Vmap (@termpoly k) v)
       end.
 
@@ -163,13 +163,13 @@ Section S.
       Vforall (@P xint k) ts.
 
     Lemma termpoly_v_eq_1 : forall x k (H : (x<=k)%nat),
-      termpoly (BVar H) = (1%Z, mxi (gt_le_S (le_lt_n_Sm H))) :: pzero (S k).
+      termpoly (BVar H) = (1%Z, mxi (NatCompat.gt_le_S (NatCompat.le_lt_n_Sm H))) :: pzero (S k).
 
     Proof. refl. Qed.
 
     Lemma termpoly_v_eq_2 :
       forall x k (H : (x<=k)%nat) (v : vector Z (S k)),
-        peval (termpoly (BVar H)) v = meval (mxi (gt_le_S (le_lt_n_Sm H))) v.
+        peval (termpoly (BVar H)) v = meval (mxi (NatCompat.gt_le_S (NatCompat.le_lt_n_Sm H))) v.
 
     Proof.
       intros x k H v. rewrite termpoly_v_eq_1. unfold pzero. unfold peval at 1.
@@ -183,7 +183,7 @@ Section S.
       intros v Hv. unfold P, f1, f2. simpl bterm_int.
       rewrite val_peval_D, termpoly_v_eq_2, meval_xi, Vnth_map.
       pattern (xint v) at 1.
-      rewrite <- (Vnth_vec_of_val xint (gt_le_S (le_lt_n_Sm Hv))).
+      rewrite <- (Vnth_vec_of_val xint (NatCompat.gt_le_S (NatCompat.le_lt_n_Sm Hv))).
       refl.
 
       intros f ts. unfold Q. intro H. unfold P, f1, f2.
