Util/List/ListUtil.v
@@ -724,8 +724,8 @@ Section remove.
 
   Proof.
     induction l; simpl; intros. contr. destruct (eq_dec a x).
-    apply le_lt_n_Sm.
-    apply length_remove. destruct H. rewrite H in n. tauto. simpl. apply lt_n_S.
+    apply NatCompat.le_lt_n_Sm.
+    apply length_remove. destruct H. rewrite H in n. tauto. simpl. apply NatCompat.lt_n_S.
     apply IHl. hyp.
   Qed.
 
@@ -956,7 +956,7 @@ Section pos.
 
     Proof.
       induction l; intro h; simpl. fo. destruct (eq_dec a x). lia.
-      apply lt_n_S. fo.
+      apply NatCompat.lt_n_S. fo.
     Qed.
 
   End def.
@@ -1653,7 +1653,7 @@ Section ith.
       | cons x m => fun i =>
         match i return i < S (length m) -> A with
 	  | O => fun _ => x
-	  | S j => fun H => ith (lt_S_n H)
+	  | S j => fun H => ith (NatCompat.lt_S_n H)
         end
     end.
 
@@ -1710,7 +1710,7 @@ Section pvalues.
     match n as n return (forall i, i < n -> A) -> list A with
       | 0 => fun _ => nil
       | S k => fun f =>
-        f 0 (Nat.lt_0_succ k) :: pvalues (fun i h => f (S i) (lt_n_S h))
+        f 0 (Nat.lt_0_succ k) :: pvalues (fun i h => f (S i) (NatCompat.lt_n_S h))
     end.
 
   Lemma pvalues_eq : forall n (f g : forall i, i < n -> A),
