Util/Relation/Iter.v
@@ -163,7 +163,7 @@ simpl; unfold compose; exists z; hyp.
 rewrite IHn in H; destruct H as [p]; exists p; intuition; auto with *.
 
 destruct H as [p]; destruct H. destruct (le_lt_eq_dec H).
-right; apply lt_n_Sm_le in l; rewrite IHn; exists p; auto with *.
+right; apply NatCompat.lt_n_Sm_le in l; rewrite IHn; exists p; auto with *.
 subst; left; unfold compose in H0; auto with *.
 Qed.
 
@@ -186,7 +186,7 @@ rewrite IHn in H; destruct H as [p]; exists p; intuition; auto with *.
 
 destruct H as [p]; destruct H.
 destruct (le_lt_eq_dec H).
-right; apply lt_n_Sm_le in l; rewrite IHn; exists p; auto with *.
+right; apply NatCompat.lt_n_Sm_le in l; rewrite IHn; exists p; auto with *.
 subst; left; unfold compose in H0; auto with *.
 simpl in H0; unfold compose in *; destruct H0 as [z]; exists z.
 split; destruct H0; auto with *.
